erasure/theories/EInlineProjections.v
@@ -422,6 +422,17 @@ Proof.
   destruct lookup_env as [[decl|]|] => //.
 Qed.
 
+Lemma lookup_inductive_pars_optimize {efl : EEnvFlags} {Σ : GlobalContextMap.t} ind :
+  wf_glob Σ ->
+  EGlobalEnv.lookup_inductive_pars Σ ind = EGlobalEnv.lookup_inductive_pars (optimize_env Σ) ind.
+Proof.
+  rewrite /lookup_inductive_pars => wf.
+  rewrite /lookup_inductive /lookup_minductive.
+  rewrite (lookup_env_optimize ind wf).
+  rewrite /GlobalContextMap.lookup_inductive /GlobalContextMap.lookup_minductive.
+  destruct lookup_env as [[decl|]|] => //.
+Qed.
+
 Lemma is_propositional_cstr_optimize {efl : EEnvFlags} {Σ : GlobalContextMap.t} ind c :
   wf_glob Σ ->
   constructor_isprop_pars_decl Σ ind c = constructor_isprop_pars_decl (optimize_env Σ) ind c.
